Implement effectful intros for lists with selectors

pulse/examples/steel/Steel.Sel.LList.fsti
@@ -3,6 +3,8 @@ module Steel.Sel.LList
 open Steel.Memory
 open Steel.SelEffect
 
+module L = FStar.List.Tot
+
 
 val cell (a:Type0) : Type0
 let t (a:Type0) = ref (cell a)
@@ -17,6 +19,9 @@ val mk_cell (n: t 'a) (d:'a)
       data c == d)
 
 
+val null_llist (#a:Type) : t a
+val is_null (#a:Type) (ptr:t a) : bool
+
 
 val llist_sl (#a:Type0) (r:t a) : slprop u#1
 val llist_sel (#a:Type0) (r:t a) : selector (list a) (llist_sl r)
@@ -28,3 +33,28 @@ let llist' #a r : vprop' =
    sel = llist_sel r}
 unfold
 let llist (#a:Type0) (r:t a) = VUnit (llist' r)
+
+[@@ __steel_reduce__]
+let v_llist (#a:Type0) (#p:vprop) (r:t a)
+  (h:rmem p{FStar.Tactics.with_tactic selector_tactic (can_be_split p (llist r) /\ True)})
+  = h (llist r)
+
+val intro_llist_nil (a:Type0)
+  : SteelSel unit vemp (fun _ -> llist (null_llist #a))
+          (requires fun _ -> True)
+          (ensures fun _ _ h1 -> v_llist #a null_llist h1 == [])
+
+val intro_llist_cons (#a:Type0) (ptr1 ptr2:t a)
+  : SteelSel unit (vptr ptr1 `star` llist ptr2)
+                  (fun _ -> llist ptr1)
+                  (requires fun h -> next (sel ptr1 h) == ptr2)
+                  (ensures fun h0 _ h1 -> v_llist ptr1 h1 == (data (sel ptr1 h0)) :: v_llist ptr2 h0)
+
+val tail (#a:Type0) (ptr:t a)
+  : SteelSel (t a) (llist ptr)
+                   (fun n -> vptr ptr `star` llist n)
+                   (requires fun _ -> ptr =!= null_llist)
+                   (ensures fun h0 n h1 ->
+                     Cons? (v_llist ptr h0) /\
+                     sel ptr h1 == mk_cell n (L.hd (v_llist ptr h0)) /\
+                     v_llist n h1 == L.tl (v_llist ptr h0))
